bedrock2/src/Examples/Swap.v
@@ -5,7 +5,7 @@ Import BinInt String.
 Local Open Scope string_scope. Local Open Scope Z_scope. Local Open Scope list_scope.
 
 Section bsearch.
-  Context {p : unique! StringNames.Syntax.parameters} {b : BasicALU.operations}.
+  Context {p : unique! StringNames_parameters} {b : BasicALU.operations}.
   Local Coercion literal (z : Z) : expr := expr.literal z.
   Local Coercion var (x : String.string) : expr := expr.var x.
 
